---
title: "[CSP-S2019 江西] 和积和"
---

$$
S(l,r)=\sum_{i=l}^r a_i\times \sum_{i=l}^r b_i
$$
$$
求 \sum_{l=1}^n \sum_{r=l}^n S(l,r)
$$
$$
求 \sum_{l=1}^n \sum_{r=l}^n (\sum_{i=l}^r a_i\times \sum_{i=l}^r b_i)
$$
$$
SA_i = \sum_{j=1}^i a_j\\
SB_i = \sum_{j=1}^i b_j
$$
$$
求 \sum_{l=1}^n \sum_{r=l}^n (SA_r-SA_{l-1})\times (SB_r-SB_{l-1})
$$
$$
求 \\
\sum_{l=1}^n \sum_{r=l}^n (SA_r*SB_r)\\
-\sum_{l=1}^n \sum_{r=l}^n (SA_r*SB_{l-1})\\
-\sum_{l=1}^n \sum_{r=l}^n (SA_{l-1}*SB_{r})\\
+\sum_{l=1}^n \sum_{r=l}^n (SA_{l-1}\times SB_{l-1})
$$
$$
SSA_i = \sum_{j=1}^i SA_j \\
SSB_i = \sum_{j=1}^i SB_j \\
SSAB_i = \sum_{j=1}^i SA_j\times SB_j 
$$
$$
求 \\
\sum_{l=1}^n  (SSAB_n-SSAB_{l-1})\\
-\sum_{l=1}^n (SSA_{n}-SSA_{l-1})\times SB_{l-1}\\
-\sum_{l=1}^n SA_{l-1}\times (SSB_{n}-SSB_{l-1})\\
+\sum_{l=1}^n (n-l+1)\times (SA_{l-1}\times SB_{l-1})
$$











